Fix encoding

src/pl/encodable.lean
@@ -4,45 +4,343 @@ Released under the Apache License 2.0 (see "License");
 Author: Bruno Bentzen
 -/
 
-import .syntax.language.basic
+import ..prime data.encodable .syntax.language.basic
 
-open nat
+open form nat list decidable 
 
 variables {σ : nat}
 
+/- encoding of propositional formulas -/
+
+@[reducible]
+def encode_form : form σ → nat
+| (atom v)   := 3^(v.1 + 1)
+|  (bot σ)   := 2
+| (impl p q) := 5^(encode_form p) * 7^(encode_form q)
+
+/- our encoding is well behaved -/
+
+def is_atom (n : nat) : Prop :=
+list.rec_on (factors n) true (λ n _ ih, if n = 3 then ih else false)
+
+def is_impl (n : nat) : Prop :=
+list.rec_on (factors n) true (λ n _ ih, if n = 5 ∨ n = 7 then ih else false)
+
+instance is_atom_dec {n : nat} : decidable (is_atom n) :=
+begin
+  induction n, simp,
+    apply is_true, trivial,
+    unfold is_atom ite, induction factors (succ n_n),
+      simp, apply is_true, trivial,
+      simp, induction (nat.decidable_eq hd 3),
+        simp, apply is_false, apply id,
+        simp, assumption
+end
+
+instance is_impl_dec {n : nat} : decidable (is_impl n) :=
+begin
+  induction n, simp,
+    apply is_true, trivial,
+    unfold is_impl ite, induction factors (succ n_n),
+      simp, apply is_true, trivial,
+      simp, induction (nat.decidable_eq hd _),
+        repeat {
+          induction or.decidable,
+            simp, apply is_false, apply id,
+            simp, assumption
+        }
+end
+
+def encode_ge_one : ∀ (p : form σ), encode_form p ≥ 1
+| (#v) := by apply nat.le_trans (succ_le_succ (zero_le 1)); apply prime_exp_le prime_three
+| (bot σ) := dec_trivial
+| (p ⊃ q) := 
+  by apply nat.le_trans (succ_le_succ (zero_le 1)); 
+  apply prime_double_exp_le prime_five prime_seven
+  (encode_ge_one p) (encode_ge_one q)
+
+def is_atom_pow_three : ∀ (n : ℕ), is_atom (3^n)
+| 0 := by unfold is_atom ite
+| (k+1) := by unfold is_atom ite; rw factors_of_exp_prime prime_three; apply is_atom_pow_three
+
+def not_atom_pow_five_seven  {n m : ℕ } : ¬ is_atom (5^(n+1) * 7^(m+1)) :=
+have ¬ 5 = 3 := dec_trivial,
+by unfold is_atom ite; rw factors_of_double_exp_prime prime_five prime_seven (le_succ 6);
+  simp; induction nat.decidable_eq _ _; simp; contradiction
+
+def min_fac_pow_of_five_seven {i j : ℕ} : min_fac (5^(i+1) * 7^(j+1)) = 5 := 
+prime_exp_mul_min_fac_is_least_prime dec_trivial prime_five prime_seven (le_add_left _ _) _ (le_add_left _ _)
+
+def is_impl_pow_of_seven : ∀ {j : ℕ}, is_impl (7^(j+1))
+| 0     :=  have h₁ : 7 > 0 := dec_trivial,
+            begin
+              unfold is_impl ite, rw factors_min_fac (prime_exp_le prime_seven),
+              simp, induction nat.decidable_eq _ _,
+                induction or.decidable,
+                  simp, cases (not_or_iff_and_not _ _).1 h_1,
+                    apply false.rec, apply right, exact prime_exp_min_fac_is_self prime_seven,
+                  simp, rw [prime_exp_min_fac_is_self prime_seven, nat.pow_one, nat.div_self h₁, factors_one], simp,
+                apply absurd h, 
+                  rw prime_exp_min_fac_is_self prime_seven, exact dec_trivial
+            end
+
+| i@(k+1) :=
+  begin
+  unfold is_impl ite, rw factors_min_fac (prime_exp_le prime_seven),
+    simp, induction nat.decidable_eq _ _,
+      induction or.decidable,
+        simp, cases (not_or_iff_and_not _ _).1 h_1,
+          apply false.rec, apply right, exact prime_exp_min_fac_is_self prime_seven,
+        simp, rw [prime_exp_min_fac_is_self prime_seven, mul_exp_div _ (lt_trans (nat.zero_lt_succ _) (prime.ge_two prime_seven))],
+        apply is_impl_pow_of_seven,
+      apply absurd h,
+        rw prime_exp_min_fac_is_self prime_seven, exact dec_trivial
+  end
+
+def is_impl_pow_of_five_seven {j : ℕ} : ∀ {i : ℕ}, is_impl (5^(i+1) * 7^(j+1))
+| 0     :=  begin
+              unfold is_impl ite, rw factors_min_fac (prime_double_exp_le prime_five prime_seven (le_add_left _ _) (le_add_left _ _)),
+              simp, induction nat.decidable_eq _ _,
+                apply false.rec, apply h, exact min_fac_pow_of_five_seven,
+                induction or.decidable,
+                  simp, cases (not_or_iff_and_not _ _).1 h_1,
+                    apply false.rec, apply left, exact min_fac_pow_of_five_seven,
+                  simp, rw min_fac_pow_of_five_seven, rw mul_exp_div_right (prime.ge_two prime_five),
+                  rw [nat.pow_zero, mul_comm, nat.mul_one],
+                  apply is_impl_pow_of_seven
+            end
+
+| i@(k+1) :=
+have h₁ : 5 < 7 := dec_trivial,
+have h₂ : min_fac (5^(i+1) * 7^(j+1)) = 5 := prime_exp_mul_min_fac_is_least_prime h₁ prime_five prime_seven (le_add_left _ _) _ (le_add_left _ _),
+  begin
+    unfold is_impl ite, rw factors_min_fac (prime_double_exp_le prime_five prime_seven (le_add_left _ _) (le_add_left _ _)),
+    simp, induction nat.decidable_eq _ _,
+      contradiction,
+      induction or.decidable,
+        simp, cases (not_or_iff_and_not _ _).1 h_1,
+          contradiction,
+        simp, rw h₂, rw mul_exp_div_right (prime.ge_two prime_five),
+        apply is_impl_pow_of_five_seven
+  end
+
+lemma is_impl_has_pow_of_five_seven : ∀ (n : ℕ), n ≠ 0 → is_impl n → ∃ (i j : ℕ), n = 5^i * 7^j
+| 0      := by intro; contradiction 
+| 1      := by intros; fapply exists.intro 0; fapply exists.intro 0; repeat {rw nat.pow_zero}; simp
+| (k+2)  :=
+  have h₁ : (k+2) / min_fac (k+2) < k+2 := factors_lemma,
+  have h₂ : (k+2) > 0 := lt_trans (zero_lt_succ 0) (le_add_left _ _),
+  begin
+    intro h, unfold is_impl ite, rw factors_min_fac (le_add_left _ _),
+    simp, induction nat.decidable_eq _ _,
+      induction or.decidable,
+        simp, simp, intro h₃,
+          have hn : ∃ (i j : ℕ), (k + 2) / min_fac (k + 2) = 5 ^ i * 7 ^ j := 
+            is_impl_has_pow_of_five_seven ((k+2) / min_fac (k+2)) (pos_div_min_fac (k+2) h₂) h₃,
+          cases hn with i h_3,
+            cases h_3 with j h_3,
+              rw (or.resolve_left h_2 h_1) at h_3,
+              fapply exists.intro i, fapply exists.intro (j+1),
+                rw [nat.pow_succ, eq.symm (nat.mul_assoc (5^i) (7^j) _), eq.symm h_3],
+                apply eq.symm, apply nat.div_mul_cancel,
+                  rw eq.symm (or.resolve_left h_2 h_1),
+                  apply min_fac_dvd,
+      induction or.decidable,
+        cases (not_or_iff_and_not _ _).1 h_2,
+          contradiction,
+        simp, intro h₃, 
+            have hn : ∃ (i j : ℕ), (k + 2) / min_fac (k + 2) = 5 ^ i * 7 ^ j :=
+              is_impl_has_pow_of_five_seven ((k+2) / min_fac (k+2)) (pos_div_min_fac (k+2) h₂) h₃,
+            cases hn with i h_3,
+              cases h_3 with j h_3,
+              rw h_1 at h_3, 
+              fapply exists.intro (i+1), fapply exists.intro j,
+                rw [nat.pow_succ, (nat.mul_assoc (5^i) _ (7^j)), nat.mul_comm 5 (7^j)],
+                rw [eq.symm (nat.mul_assoc (5^i) (7^j) _), eq.symm h_3],
+                apply eq.symm, apply nat.div_mul_cancel,
+                  rw eq.symm h_1,
+                  apply min_fac_dvd
+  end
+
+-- our decoding function is well-founded
+
+lemma impl_five_count_lt (n ≠ 0) : is_impl n → count 5 (factors n) < n :=
+have h₁ : 5 < 7 := dec_trivial, 
+begin
+  intro h₂, cases is_impl_has_pow_of_five_seven n H h₂ with i h₂, cases h₂ with j h₂,
+    rw h₂, rw count_exps_factors_right prime_five prime_seven h₁,
+    cases nat.decidable_eq i 0,
+      cases nat.decidable_eq j 0,
+        apply lt_trans,
+          apply exp_lt_pow 5 dec_trivial,
+            rw nat.mul_comm, apply lt_mul_of_gt_one_left, 
+              apply pow_lt_of_self_lt,
+                exact dec_trivial, apply pos_iff_ne_zero.2 h_1,
+              apply lt_trans (zero_lt_succ 0),
+                apply pow_lt_of_self_lt,
+                  exact dec_trivial, apply pos_iff_ne_zero.2 h,
+        rw h_1, rw nat.pow_zero, rw nat.mul_one,
+        apply exp_lt_pow, exact dec_trivial,
+      rw h, rw nat.pow_zero, rw nat.mul_comm, rw nat.mul_one,
+      apply pow_ge_one, exact dec_trivial
+end
+
+lemma impl_seven_count_lt (n ≠ 0) : is_impl n → count 7 (factors n) < n :=
+have h₁ : 5 < 7 := dec_trivial, 
+begin
+  intro h₂, cases is_impl_has_pow_of_five_seven n H h₂ with i h₂, cases h₂ with j h₂,
+    rw h₂, rw count_exps_factors_left prime_five prime_seven h₁,
+    cases nat.decidable_eq j 0,
+      cases nat.decidable_eq i 0,
+        apply lt_trans,
+          apply exp_lt_pow 7 dec_trivial,
+            apply lt_mul_of_gt_one_left,
+              apply pow_lt_of_self_lt,
+                exact dec_trivial, apply pos_iff_ne_zero.2 h_1,
+              apply lt_trans (zero_lt_succ 0),
+                apply pow_lt_of_self_lt,
+                  exact dec_trivial, apply pos_iff_ne_zero.2 h,
+        rw h_1, rw nat.pow_zero, rw nat.mul_comm, rw nat.mul_one,
+        apply exp_lt_pow, exact dec_trivial,
+      rw h, rw nat.pow_zero, rw nat.mul_one,
+      apply pow_ge_one, exact dec_trivial
+end
+
+/- decoding of propositional formulas -/
+
+@[reducible]
+def decode_form (σ : nat) : nat → option (form σ)
+|   0     := none 
+|   1     := none 
+|   2     := some (bot σ)
+| n@(k+3) := 
+  if is_atom n 
+  then
+    if h : count 3 (factors n) - 1 < σ
+    then 
+      option.some (#⟨count 3 (factors n) - 1,h⟩) 
+    else
+      none
+  else if h : is_impl n 
+    then
+      have count 5 (factors n) < n := impl_five_count_lt _ (succ_ne_zero _) h,
+      have count 7 (factors n) < n := impl_seven_count_lt _ (succ_ne_zero _) h,
+      option.rec_on (decode_form (count 5 (factors n))) none
+      (λ p, option.rec_on (decode_form (count 7 (factors n))) none 
+        (λ q, some (p ⊃ q)) )
+    else none 
+
+def decode_form_lemma {n : ℕ} (h : n ≥ 3) :
+  decode_form σ n =
+    if is_atom n 
+    then
+      if h₁ : count 3 (factors n) - 1 < σ 
+      then 
+        option.some (#⟨count 3 (factors n) - 1,h₁⟩) 
+      else
+        none
+    else if h₂ : is_impl n 
+      then
+        have count 5 (factors n) < n := impl_five_count_lt _ (by intro hn; cases hn; apply absurd h (not_lt_zero 2)) h₂,
+        have count 7 (factors n) < n := impl_seven_count_lt _ (by intro hn; cases hn; apply absurd h (not_lt_zero 2)) h₂,
+        option.rec_on (decode_form σ (count 5 (factors n))) none
+        (λ p, option.rec_on (decode_form σ (count 7 (factors n))) none 
+          (λ q, some (p ⊃ q)) )
+      else none 
+ :=
+by cases le.dest h; unfold dite; rw h_1.symm; rw nat.add_comm 3 w at *; unfold decode_form ite dite
+
+/- encoding of propositional formulas preserves data -/
+
+-- falsum
+
+def encodek_bot : decode_form σ (encode_form (⊥ : form σ)) = some ⊥ :=
+by unfold decode_form
+
+-- atom
+
+def encodek_atom (v : var σ) : decode_form σ (encode_form (#v)) = some (#v) :=
+match v with 
+⟨ n , h ⟩  := begin 
+                unfold encode_form, induction n, 
+                  simp, unfold decode_form ite,
+                  rw nat.add_comm 0 3 at *, simp at *,
+                    induction is_atom_dec,
+                    apply absurd (is_atom_pow_three 1),
+                      rw nat.pow_one 3, assumption,
+                    simp at *, unfold dite,
+                    induction nat.decidable_lt _ _,
+                      simp, rw nat.add_zero 3 at *,
+                      rw factors_of_prime prime_three at *,
+                        simp at *, cases eq_or_lt_of_le h_2,
+                          rw h_3 at *, apply absurd h, apply lt_irrefl,
+                          apply nat.lt_asymm h, assumption,
+                      simp, apply fin.eq_of_veq, unfold fin.val,
+                        rw factors_of_prime prime_three, simp,
+
+                  have hle : 3^((succ n_n)+1) ≥ 3 := le_pow_self (succ_le_succ (nat.zero_le 2)),
+                  simp, rw decode_form_lemma hle, unfold ite, 
+                  induction is_atom_dec,
+                    apply absurd (is_atom_pow_three _) h_1,
+                    unfold dite, induction nat.decidable_lt _ _,
+                      simp, rw factors_of_exp_prime prime_three at *,
+                        apply h_2, rw count_cons_self, rw count_exp_factors prime_three,
+                        simp, repeat {assumption},
+                      simp, apply fin.eq_of_veq, unfold fin.val,
+                        rw count_exp_factors prime_three, simp
+              end 
+end
+
+lemma imp_encode_ge_three {p q : form σ} : 5^(encode_form p) * 7^(encode_form q) ≥ 3 :=
+have h₁ : 3 ≤ 5 := dec_trivial,
+have h₂ : 1 ≤ 5 := dec_trivial,
+have h₃ : 1 ≤ 7 := dec_trivial,
+begin
+  apply le_trans h₁,
+    apply le_trans (pow_le_no_pow h₂ (encode_ge_one p)),
+        rw nat.mul_comm, apply le_mul_of_ge_one_left'',
+          apply le_trans h₃ (pow_le_no_pow h₃ (encode_ge_one q)),
+          apply le_trans (nat.zero_le 5), apply (pow_le_no_pow h₂ (encode_ge_one p))
+end
+
+-- implication
+
+def encodek_impl {p q : form σ} :
+  decode_form σ (encode_form p) = some p → 
+  decode_form σ (encode_form q) = some q →
+  decode_form σ (encode_form (p ⊃ q)) = some (p ⊃ q) :=
+begin
+  intros hp hq, unfold encode_form,
+  have hle : 5^(encode_form p) * 7^(encode_form q) ≥ 3 := imp_encode_ge_three,
+  rw decode_form_lemma hle, unfold ite, 
+  induction is_atom_dec,
+    simp, induction is_impl_dec,
+      cases le.dest (encode_ge_one p), rw nat.add_comm at h_2,
+        cases le.dest (encode_ge_one q), rw nat.add_comm at h_3,
+          unfold dite, simp, 
+        apply h_1, induction h_2, induction h_3,
+          apply is_impl_pow_of_five_seven,
+      unfold dite,
+        rw count_exps_factors_right prime_five prime_seven,
+        rw count_exps_factors_left prime_five prime_seven,
+        rw [hp,hq], repeat {apply le_succ},
+    apply absurd h, 
+      cases le.dest (encode_ge_one p), rw nat.add_comm at h_1,
+      cases le.dest (encode_ge_one q), rw nat.add_comm at h_2,
+        induction h_1, induction h_2,
+          apply not_atom_pow_five_seven
+end
+
+-- putting all the pieces together
+
+def encodek_form : ∀ (p : form σ), decode_form σ (encode_form p) = some p
+| (atom v)   := encodek_atom v
+|  (bot σ)   := encodek_bot
+| (impl p q) := encodek_impl (encodek_form p) (encodek_form q)
+
 /- enumeration of all propositional atoms -/
 
-class encodable (α : Type*) :=
-(encode : α → nat) (decode : nat → option α) (encodek : ∀ a, decode (encode a) = some a)
+instance of_form : encodable (form σ) :=
+⟨ encode_form , decode_form σ , encodek_form ⟩ 
 
--- TODO: --import factors and other operations from mathlib
-
-instance of_form : encodable (form σ) := sorry
-
-def no_code_is_zero : ∀ p : form σ, encodable.encode p ≥ 1 := sorry 
-
-/-
-def encode_form : form σ → nat
-|  (#v) := 3^(v.1 + 1)
-|   ⊥    := 2
-| (p ⊃ q) := 5^(encode_form p) * 7^(encode_form q)
-
-noncomputable def no_of_occurr : list nat → nat → nat
-| []     b := 0
-| (a::l) b := if a = b then no_of_occurr l b + 1 else no_of_occurr l b
-
-def decode_atom (n : nat) : Prop :=
-list.rec_on (factors n) true (λ n _ ih, if n = 2 then ih else false)
-
-def decode_impl (n : nat) : Prop :=
-list.rec_on (factors n) true (λ n _ ih, if n ≠ 3 ∨ n ≠ 5 then false else ih)
-
-noncomputable def decode_form : nat → option (form σ)
-|   0   := none 
-|   1   := none 
-|   2   := some ⊥
-| (k+3) := let n := k+3 in
-  if decode_atom n then dite (pred (no_of_occurr (factors n) 3) < σ) (λ h , option.some (#⟨_,h⟩ )) (λ _, none) else
-  if decode_impl n then option.some (_ ⊃ _) -- decode (no_of_occurr (factors n) 5)
-  else none
--/
+def no_code_is_zero : ∀ p : form σ, encodable.encode p ≥ 1 := λ p, encode_ge_one p 
