src/misc.lean
@@ -6,6 +6,8 @@ Author: Bruno Bentzen
 
 -- some general lemmas used in this project
 
+import logic.basic
+
 def contrap {p q : Prop} : 
   (p → q) ↔ (¬ q → ¬ p) :=
 iff.intro (λ f nq p, nq (f p))
@@ -13,5 +15,9 @@ iff.intro (λ f nq p, nq (f p))
 
 def not_contrap {p q : Prop} : 
   (¬ q → ¬ p) → (p → q) :=
+--not_imp_not.1
 contrap.2
 
+--variables p q : Prop
+
+--#check @not_imp_not q p classical.
